InstructionDecoder.fst
@@ -8,37 +8,30 @@ open Cpu
 open Memory
 open Value
 
-/// ================
-/// Type definitions
-/// ================
-(*
- * Instruction operand, representing the target of a read or write by a
- * normal instruction (not a store or load).
- *)
+
+
+
+/// ====================
+/// Instruction operands
+/// ====================
+///
+/// We now begin in earnest by describing how instruction operands are handled.
+///
+/// An instruction operand represents the target of a read or write
+/// to the register file (or from an immediate).
 type operand =
   | PC
   | Register: n:nat -> operand
   | Immediate: n:Cpu.word -> operand
 
-(*
- * Storage operation, representing a load or store from memory.
- *)
-type storage_operation =
-  | Load: address:nat -> dest:nat -> storage_operation
-  | Store: address:nat -> src:nat -> storage_operation
+/// -----
+/// Reads
+/// -----
 
-(*
- * A cache policy function, specifying what a given storage operation does
- * to a system's cache state.
- *)
-type cache_policy (n:memory_size) =
-       (cache_state n) -> storage_operation -> (cache_state n)
-
-
-/// ========================
-/// Register file operations
-/// ========================
-let rec get_operands (#n #r: memory_size) (operands:list operand) (state:systemState #n #r): rv:(list (maybeBlinded #word)){FStar.List.length rv = FStar.List.length operands} =
+/// The first object of analysis is the function ``get_operands``, that will
+/// take a list of input operands and extract them from the system state.
+let rec get_operands (#n #r: memory_size) (operands:list operand) (state:systemState #n #r):
+    rv:(list (maybeBlinded #word)){FStar.List.length rv = FStar.List.length operands} =
   match operands with
     | Nil -> Nil
     | hd :: tl -> (match hd with
@@ -49,235 +42,101 @@ let rec get_operands (#n #r: memory_size) (operands:list operand) (state:systemS
                   | Immediate n -> Clear n
                 ) :: get_operands tl state
 
-let get_operands_with_one_operand_on_redacted_input_has_redacted_output (#n #r: memory_size) (op: operand) (state:systemState #n #r):
+/// We start by proving that operand extraction preserves redaction.
+///
+/// We do this by induction.  It is convenient to first prove that extraction
+/// of just one operand preserves redaction:
+let get_operands_with_one_operand_on_redacted_input_has_redacted_output (#n #r: memory_size)
+    (op: operand) (state:systemState #n #r):
   Lemma (ensures get_operands [op] (redact_system state) = redact_list (get_operands [op] state) 0uL) =
   let head = FStar.List.Tot.hd (get_operands [op] state) in
   let head_of_redacted = FStar.List.Tot.hd (get_operands [op] (redact_system state)) in
   match op with
     | PC -> ()
     | Register n -> (
-                   lists_are_equivalent_to_their_redaction _ state.registers 0uL;
-                   equal_lists_are_equivalent _ (redact_system state).registers  (redact_list state.registers 0uL);
-                   equivalent_lists_have_equal_lengths state.registers (redact_system state).registers;
-                   if n >= FStar.List.length state.registers then ()
-                   else ()
+        lists_are_equivalent_to_their_redaction _ state.registers 0uL;
+        equal_lists_are_equivalent _ (redact_system state).registers  (redact_list state.registers 0uL);
+        equivalent_lists_have_equal_lengths state.registers (redact_system state).registers;
+        if n >= FStar.List.length state.registers then () else ()
       )
     | Immediate n -> ()
 
-let rec get_operands_on_redacted_input_has_redacted_output (#n #r: memory_size) (operands:list operand) (state:systemState #n #r):
-  Lemma (ensures get_operands operands (redact_system state) = redact_list (get_operands operands state) 0uL)
+/// In the inductive case we show that the first operand in the list will be
+/// redacted as above, and then recurse by repeating this for the tail of the
+/// operand list.
+let rec get_operands_on_redacted_input_has_redacted_output (#n #r: memory_size)
+    (operands:list operand) (state:systemState #n #r):
+  Lemma (ensures get_operands operands (redact_system state)
+                 = redact_list (get_operands operands state) 0uL)
         [SMTPat (get_operands operands (redact_system state))] =
   (
     match operands with
       | Nil -> ()
-      | hd :: tl -> ( let head = FStar.List.Tot.hd (get_operands operands state) in
-                    let head_of_redacted = FStar.List.Tot.hd (get_operands operands (redact_system state)) in
+      | hd :: tl -> (
+          let head = FStar.List.Tot.hd (get_operands operands state) in
+          let head_of_redacted = FStar.List.Tot.hd (get_operands operands (redact_system state)) in
 
-                    get_operands_with_one_operand_on_redacted_input_has_redacted_output hd state;
-                    assert(redact head 0uL = head_of_redacted);
+          get_operands_with_one_operand_on_redacted_input_has_redacted_output hd state;
+          assert(redact head 0uL = head_of_redacted);
 
-                    let redacted_head = redact head 0uL in
+          let redacted_head = redact head 0uL in
 
-                    get_operands_on_redacted_input_has_redacted_output tl state;
-                    assert(get_operands tl (redact_system state) = redact_list (get_operands tl state) 0uL);
-                    assert((head_of_redacted :: (get_operands tl (redact_system state)))
-                         = (redacted_head :: (redact_list (get_operands tl state) 0uL)))
-                  )
+          get_operands_on_redacted_input_has_redacted_output tl state;
+          assert(get_operands tl (redact_system state) = redact_list (get_operands tl state) 0uL);
+          assert((head_of_redacted :: (get_operands tl (redact_system state)))
+            = (redacted_head :: (redact_list (get_operands tl state) 0uL)))
+        )
 )
 
-let rec get_operands_on_equivalent_inputs_has_equivalent_output (#m #q #n #r: memory_size) (operands:list operand) (state1: systemState #m #q) (state2:systemState #n #r):
+/// We then prove that extracting operands from the state also preserves
+/// equivalence, though in this case we jump to the inductive proof directly.
+let rec get_operands_on_equivalent_inputs_has_equivalent_output (#m #q #n #r: memory_size)
+    (operands:list operand) (state1: systemState #m #q) (state2:systemState #n #r):
   Lemma (requires (equiv_system state1 state2))
         (ensures  (equiv_list (get_operands operands state1)
                               (get_operands operands state2)))
   = match operands with
       | Nil -> ()
-      | hd :: tl -> (let result_hd1, result_hd2 = match hd with
-                    | PC -> (
-                         let head1 = FStar.List.Tot.hd (get_operands operands state1) in
-                         let head2 = FStar.List.Tot.hd (get_operands operands state2) in
-                         equal_values_are_equivalent Cpu.word head1 head2;
-                         head1, head2
-                         )
-                    | Register n -> (
-                        assert(equiv_list state1.registers state2.registers);
-                        equivalent_lists_have_equal_lengths state1.registers state2.registers;
-                        assert((FStar.List.length state1.registers) = (FStar.List.length state2.registers));
-                        if n < FStar.List.length state1.registers then (
-                          equivalent_lists_have_equivalent_values _ state1.registers state2.registers n )
-                        else ();
-
-                        FStar.List.Tot.hd (get_operands operands state1), FStar.List.Tot.hd (get_operands operands state2)
-                        )
-                    | Immediate n -> (Clear n, Clear n) in
-
-                    assert(equiv result_hd1 result_hd2);
-                    get_operands_on_equivalent_inputs_has_equivalent_output tl state1 state2
+      | hd :: tl -> (
+          let result_hd1, result_hd2 =
+            match hd with
+             | PC -> (
+                  let head1 = FStar.List.Tot.hd (get_operands operands state1) in
+                  let head2 = FStar.List.Tot.hd (get_operands operands state2) in
+                  equal_values_are_equivalent Cpu.word head1 head2;
+                  head1, head2
+               )
+             | Register n -> (
+                  assert(equiv_list state1.registers state2.registers);
+                  equivalent_lists_have_equal_lengths state1.registers state2.registers;
+                  if n < FStar.List.length state1.registers then (
+                       equivalent_lists_have_equivalent_values _ state1.registers state2.registers n
                   )
+                  else ();
 
-/// ====================
-/// Instruction decoding
-/// ====================
-
-type decodedInstruction = { opcode: nat; input_operands: list operand; output_operands: list operand }
-
-type decoder = (inst:word) -> decodedInstruction
-
-type instruction_result (di:decodedInstruction) = {
-  register_writes: (vals:(list (maybeBlinded #word)){FStar.List.length vals = FStar.List.length di.output_operands});
-  memory_ops   :(list storage_operation)
-  }
-
-/// =================
-/// Memory operations
-/// =================
-
-let equiv_storage_operation (lhs rhs: storage_operation) =
-  match lhs, rhs with
-    | (Load la ld), (Load ra rd) -> (la = ra /\ ld = rd)
-    | (Store la ls), (Store ra rs) -> (la = ra /\ ls = rs)
-    | _, _ -> False
-
-let rec equiv_storage_operations (lhs rhs: list storage_operation) =
-  match lhs, rhs with
-    | lh :: lt, rh :: rt -> (equiv_storage_operation lh rh) /\ equiv_storage_operations lt rt
-    | [], [] -> True
-    | _, _ -> False
-
-let equal_storage_operations_are_equivalent (lhs rhs: storage_operation):
-  Lemma (requires lhs = rhs)
-        (ensures  (equiv_storage_operation lhs rhs)) =
-  ()
-
-let rec equal_storage_operation_lists_are_equivalent (lhs rhs: list storage_operation):
-  Lemma (requires lhs = rhs)
-        (ensures equiv_storage_operations lhs rhs) =
-  match lhs, rhs with
-    | hl :: tl, hr :: tr -> (
-         equal_storage_operations_are_equivalent hl hr;
-         equal_storage_operation_lists_are_equivalent tl tr
+                  FStar.List.Tot.hd (get_operands operands state1),
+                    FStar.List.Tot.hd (get_operands operands state2)
+               )
+             | Immediate n -> (Clear n, Clear n) in
+                 assert(equiv result_hd1 result_hd2);
+                 get_operands_on_equivalent_inputs_has_equivalent_output tl state1 state2
       )
-    | _ -> ()
-
-let storage_operation_equivalence_is_symmetric (lhs rhs: storage_operation):
-  Lemma (requires (equiv_storage_operation lhs rhs))
-        (ensures  (equiv_storage_operation rhs lhs)) =
-  ()
-
-let rec storage_operation_list_equivalence_is_symmetric (lhs rhs: list storage_operation):
-  Lemma (requires (equiv_storage_operations lhs rhs))
-        (ensures  (equiv_storage_operations rhs lhs)) =
-  match lhs, rhs with
-   | hl :: tl, hr :: tr -> (
-        storage_operation_equivalence_is_symmetric hl hr;
-        storage_operation_list_equivalence_is_symmetric tl tr
-     )
-   | _ -> ()
-
-let storage_operation_equivalence_is_transitive (lhs mid rhs: storage_operation):
-  Lemma (requires (equiv_storage_operation lhs mid) /\ (equiv_storage_operation mid rhs))
-        (ensures  (equiv_storage_operation lhs rhs)) =
-  ()
-
-let rec storage_operation_list_equivalence_is_transitive (lhs mid rhs: list storage_operation):
-  Lemma (requires (equiv_storage_operations lhs mid) /\ (equiv_storage_operations mid rhs))
-        (ensures  (equiv_storage_operations lhs rhs)) =
-  match lhs, mid, rhs with
-   | hl :: tl, hm :: tm, hr :: tr -> (
-        storage_operation_equivalence_is_transitive hl hm hr;
-        storage_operation_list_equivalence_is_transitive tl tm tr
-     )
-   | _ -> ()
-
-let rec equivalent_storage_operation_lists_have_equal_length (lhs rhs: list storage_operation):
-  Lemma (requires equiv_storage_operations lhs rhs)
-        (ensures (FStar.List.length lhs) = (FStar.List.length rhs)) =
-  match lhs, rhs with
-    | hl :: tl, hr :: tr -> equivalent_storage_operation_lists_have_equal_length tl tr
-    | _, _ -> ()
-
-/// ===========================
-/// Computation by instructions
-/// ===========================
-
-let equiv_result (#di:decodedInstruction) (lhs rhs:(instruction_result di)) =
-    (equiv_list lhs.register_writes rhs.register_writes)
-  /\ (equiv_storage_operations lhs.memory_ops rhs.memory_ops)
-
-let equal_results_are_equivalent (#di:decodedInstruction) (lhs rhs:(instruction_result di)):
-  Lemma (requires lhs = rhs)
-        (ensures  equiv_result lhs rhs)
-  = equal_lists_are_equivalent word lhs.register_writes rhs.register_writes;
-    equal_storage_operation_lists_are_equivalent lhs.memory_ops rhs.memory_ops
-
-let result_equivalence_is_symmetric (#di:decodedInstruction) (lhs rhs:(instruction_result di)):
-  Lemma (requires equiv_result lhs rhs)
-        (ensures equiv_result rhs lhs) =
-  list_equivalence_is_symmetric word lhs.register_writes rhs.register_writes;
-  storage_operation_list_equivalence_is_symmetric lhs.memory_ops rhs.memory_ops
-
-let result_equivalence_is_transitive (#di:decodedInstruction) (lhs mid rhs:(instruction_result di)):
-  Lemma (requires (equiv_result lhs mid) /\ (equiv_result mid rhs))
-        (ensures  (equiv_result lhs rhs)) =
-  list_equivalence_is_transitive word lhs.register_writes mid.register_writes rhs.register_writes;
-  storage_operation_list_equivalence_is_transitive lhs.memory_ops mid.memory_ops rhs.memory_ops
-
-type instruction_input (#n #r: memory_size) (di:decodedInstruction) =
-     pre:(list (maybeBlinded #word)){(exists(s: systemState #n #r). pre = get_operands di.input_operands s)
-                                    /\ FStar.List.length pre = FStar.List.length di.input_operands}
 
 
-let redacted_instruction_inputs_are_instruction_inputs  (#n #r: memory_size) (di:decodedInstruction) (pre:instruction_input #n #r di): instruction_input #n #r di
-  = assert(exists (s:systemState). (pre = get_operands #n #r di.input_operands s /\
-             (get_operands #n #r di.input_operands (redact_system s) = redact_list (get_operands di.input_operands s) 0uL  )  ) );
-    redact_list pre 0uL
-
-type decoder_output (d:decoder) = (di:decodedInstruction{exists(inst:word). di = d inst})
-
-type instruction_semantics (#n #r: memory_size) (d:decoder) = (di: decoder_output d) -> (pre:instruction_input #n #r di) -> instruction_result di
-
-let is_redacting_equivalent_instruction_semantics_somewhere
-      (#n #r: memory_size)
-      (d:decoder)
-      (s:instruction_semantics #n #r d)
-      (inst:word)
-      (input:instruction_input #n #r (d inst)) =
-    redaction_preserves_length word input 0uL;
-    let redacted_input = redacted_instruction_inputs_are_instruction_inputs (d inst) input in
-    (equiv_result (s (d inst) input) (s (d inst) redacted_input))
-
-let is_redacting_equivalent_instruction_semantics_everywhere (#n #r: memory_size) (d:decoder) (s:instruction_semantics #n #r d) =
-    forall (inst:word) (pre:instruction_input #n #r (d inst)).
-                is_redacting_equivalent_instruction_semantics_somewhere d s inst pre
-
-let redacting_equivalent_instruction_semantics_on_equivalent_inputs_yields_equivalent_results_somewhere
-      (#n #r: memory_size)
-      (d:decoder)
-      (s:instruction_semantics #n #r d)
-      (inst:word)
-      (input1 input2:instruction_input #n #r (d inst)):
-  Lemma (requires (is_redacting_equivalent_instruction_semantics_everywhere d s) /\ (equiv_list input1 input2))
-        (ensures  equiv_result (s (d inst) input1) (s (d inst) input2)) =
-  let result1 = (s (d inst) input1) in
-  let result2 = (s (d inst) input2) in
-  let redacted_result1 = (s (d inst) (redact_list input1 0uL)) in
-  let redacted_result2 = (s (d inst) (redact_list input2 0uL)) in
-
-  equivalent_lists_have_equal_redactions word input1 input2 0uL;
-  assert(redacted_result1 = redacted_result2);
-  equal_results_are_equivalent redacted_result1 redacted_result2;
-
-  result_equivalence_is_symmetric result2 redacted_result1;
-
-  assert(equiv_result result1 redacted_result1);
-  assert(equiv_result redacted_result1 result2);
-
-  result_equivalence_is_transitive result1 redacted_result1 result2;
-  assert(equiv_result result1 result2)
-
-/// ===============
-/// List operations
-/// ===============
-
+/// ------
+/// Writes
+/// ------
+///
+/// Next we look at how to write operands.  First we will define some utility functions.
+///
+/// The first operation that we will do is to take a list and replace a single element
+/// of a list with the corresponding element of another list (if it exists).
+///
+/// For example:
+///
+///   .. example:
+///
+///     mux_list_single [1,2,3] [4,5,6] 1 == [1,5,6]
 let rec mux_list_single (a:list(maybeBlinded #word)) (b:list(maybeBlinded #word)) (n:nat):
         list(maybeBlinded #word)
   = match a, b with
@@ -290,6 +149,15 @@ let rec mux_list_single (a:list(maybeBlinded #word)) (b:list(maybeBlinded #word)
                               else
                                 hd2 :: tl1
 
+
+/// Then we do the same thing with a whole list of elements to replace.
+let rec mux_list (a:list (maybeBlinded #word)) (b:(list (maybeBlinded #word))) (which_b:list nat):
+    Tot (list (maybeBlinded #word)) (decreases which_b) =
+  match which_b with
+    | Nil -> a
+    | index_to_change :: tl -> mux_list (mux_list_single a b index_to_change) b tl
+
+/// Then the same again replacing the list element with a specific value.
 let rec replace_list_value (orig:list(maybeBlinded #word)) (n:nat) (v:maybeBlinded #word):
         r:(list(maybeBlinded #word)){FStar.List.length r = FStar.List.length orig}
     = match orig with
@@ -300,15 +168,22 @@ let rec replace_list_value (orig:list(maybeBlinded #word)) (n:nat) (v:maybeBlind
                    else
                      v :: tl
 
-let rec replacing_in_equivalent_lists_with_equivalent_value_yields_equivalent_lists (orig1 orig2:list(maybeBlinded #word)) (n:nat) (v1 v2:maybeBlinded #word):
+/// We then show that replacing a list value preserves equivalence.
+let rec replacing_in_equivalent_lists_with_equivalent_value_yields_equivalent_lists
+    (orig1 orig2:list(maybeBlinded #word)) (n:nat) (v1 v2:maybeBlinded #word):
   Lemma (requires (equiv_list orig1 orig2) /\ (equiv v1 v2))
         (ensures (equiv_list (replace_list_value orig1 n v1) (replace_list_value orig2 n v2))) =
   match n, orig1, orig2 with
     | 0, _, _ -> ()
-    | _, h1 :: t1, h2 :: t2 -> replacing_in_equivalent_lists_with_equivalent_value_yields_equivalent_lists t1 t2 (n-1) v1 v2
+    | _, h1 :: t1, h2 :: t2 ->
+         replacing_in_equivalent_lists_with_equivalent_value_yields_equivalent_lists
+           t1 t2 (n-1) v1 v2
     | _ -> ()
 
-let rec replacing_then_reading_yields_original_value (orig: list (maybeBlinded #word)) (v:maybeBlinded #word) (n:nat):
+/// We then show that replacing a list value and reading it back yields the
+/// value that we wrote.
+let rec replacing_then_reading_yields_original_value
+    (orig: list (maybeBlinded #word)) (v:maybeBlinded #word) (n:nat):
   Lemma (requires n < FStar.List.length orig)
         (ensures FStar.List.Tot.index (replace_list_value orig n v) n = v)
     = match n, orig with
@@ -316,7 +191,11 @@ let rec replacing_then_reading_yields_original_value (orig: list (maybeBlinded #
       | 0, _ -> ()
       | _, hd :: tl -> replacing_then_reading_yields_original_value tl v (n-1)
 
-let set_one_operand (#n #r: memory_size) (operand:operand) (value:maybeBlinded #word) (state:systemState #n #r): systemState #n #r =
+/// Now that we have these utility functions, we can use them to write output
+/// to the machine state.  First a single operand:
+let set_one_operand (#n #r: memory_size)
+      (operand:operand) (value:maybeBlinded #word) (state:systemState #n #r):
+      systemState #n #r =
     match operand with
       | PC -> (match value with
                | Clear v -> if FStar.UInt64.v v < FStar.List.length state.memory then
@@ -332,7 +211,8 @@ let set_one_operand (#n #r: memory_size) (operand:operand) (value:maybeBlinded #
                        state
       | Immediate n -> state
 
-let setting_and_getting_one_non_faulting_operand_value_yields_original_value (#n #r: memory_size) (operand:operand) (value:maybeBlinded #word) (state:systemState #n #r):
+let setting_and_getting_one_non_faulting_operand_value_yields_original_value (#n #r: memory_size)
+    (operand:operand) (value:maybeBlinded #word) (state:systemState #n #r):
   Lemma (requires ~(match operand with
                      | PC -> (match value with
                               | Blinded v -> True
@@ -345,14 +225,15 @@ let setting_and_getting_one_non_faulting_operand_value_yields_original_value (#n
     | PC -> ()
     | Register n -> replacing_then_reading_yields_original_value state.registers value n
 
-
+/// As usual, we then show that writing equivalent operands preserves equivalence.
 let setting_single_equivalent_operand_values_on_equivalent_systems_yields_equivalent_systems
     (#n #r: memory_size)
     (operand       :operand)
     (value1 value2 :(maybeBlinded #word))
     (state1 state2 :systemState #n #r):
     Lemma (requires (equiv_system state1 state2) /\ (equiv value1 value2))
-          (ensures  (equiv_system (set_one_operand operand value1 state1) (set_one_operand operand value2 state2))) =
+          (ensures  (equiv_system (set_one_operand operand value1 state1)
+                                  (set_one_operand operand value2 state2))) =
     match operand with
       | PC -> (match value1, value2 with
                | Clear v1, Clear v2 -> (
@@ -367,12 +248,17 @@ let setting_single_equivalent_operand_values_on_equivalent_systems_yields_equiva
           equivalent_lists_have_equal_lengths state1.registers state2.registers;
           if n >= FStar.List.length state1.registers then ()
           else
-            replacing_in_equivalent_lists_with_equivalent_value_yields_equivalent_lists state1.registers state2.registers n value1 value2
+            replacing_in_equivalent_lists_with_equivalent_value_yields_equivalent_lists
+              state1.registers state2.registers n value1 value2
         )
       | Immediate n -> ()
 
-
-let rec set_operands (#n #r: memory_size) (operands:list operand) (values:(list (maybeBlinded #word)){FStar.List.length operands = FStar.List.length values}) (state:systemState #n #r): systemState #n #r =
+/// Then multiple operands:
+let rec set_operands (#n #r: memory_size)
+    (operands:list operand)
+    (values:(list (maybeBlinded #word)){FStar.List.length operands = FStar.List.length values})
+    (state:systemState #n #r):
+        systemState #n #r =
     match operands, values with
       | o :: tl_o, v :: tl_v -> set_operands tl_o tl_v (set_one_operand o v state)
       | _ -> state
@@ -385,50 +271,172 @@ let rec setting_equivalent_operand_values_on_equivalent_systems_yields_equivalen
     (values2:(list (maybeBlinded #word)){FStar.List.length operands = FStar.List.length values2})
     (state1: systemState #n #r)  (state2 :systemState #n #r):
     Lemma (requires (equiv_system state1 state2) /\ (equiv_list values1 values2))
-          (ensures  (equiv_system (set_operands operands values1 state1) (set_operands operands values2 state2))) =
+          (ensures  (equiv_system (set_operands operands values1 state1)
+                    (set_operands operands values2 state2))) =
     match operands, values1, values2 with
       | ho :: to, hv1 :: tv1, hv2 :: tv2 -> (
           assert(equiv hv1 hv2);
 
           let applied_head1 = set_one_operand ho hv1 state1 in
           let applied_head2 = set_one_operand ho hv2 state2 in
-          setting_single_equivalent_operand_values_on_equivalent_systems_yields_equivalent_systems ho hv1 hv2 state1 state2;
+          setting_single_equivalent_operand_values_on_equivalent_systems_yields_equivalent_systems
+            ho hv1 hv2 state1 state2;
           assert(equiv_system applied_head1 applied_head2);
 
           let applied_tail1 = (set_operands to tv1 applied_head1) in
           let applied_tail2 = (set_operands to tv2 applied_head2) in
-          setting_equivalent_operand_values_on_equivalent_systems_yields_equivalent_systems to tv1 tv2 applied_head1 applied_head2;
+          setting_equivalent_operand_values_on_equivalent_systems_yields_equivalent_systems
+            to tv1 tv2 applied_head1 applied_head2;
           assert(equiv_system applied_tail1 applied_tail2)
         )
       | _ -> ()
 
 
-let complete_one_memory_transaction (#n #r: memory_size) (op:storage_operation) (pre:systemState #n #r) (cp:cache_policy n): systemState #n #r =
-  match op with
-      | Load address register -> if register < FStar.List.length pre.registers
-                                    && address < FStar.List.length pre.memory then
-                                    { pre with registers = replace_list_value pre.registers register (FStar.List.Tot.index pre.memory address);
-                                               cache_lines = cp pre.cache_lines op }
-                                 else pre
-      | Store address register -> if register < FStar.List.length pre.registers
-                                    && address < FStar.List.length pre.memory then
-                                    { pre with memory = replace_list_value pre.memory address (FStar.List.Tot.index pre.registers register);
-                                               cache_lines = cp pre.cache_lines op }
-                                 else pre
 
-let rec complete_memory_transactions (#n #r: memory_size) (op:list storage_operation) (pre:systemState #n #r) (cp:cache_policy n) =
+/// =================
+/// Memory operations
+/// =================
+///
+/// Now we look at memory operations.
+///
+/// These are represented differently from instruction operands, because in
+/// a real processor they would handled by the load-store unit, which can't
+/// immediately read or write a value from memory: it always takes at least
+/// one cycle.
+type memory_operation =
+  | Load: address:nat -> dest:nat -> memory_operation
+  | Store: address:nat -> src:nat -> memory_operation
+
+
+/// We also need to deal with caches.  In this case we don't want to specify
+/// concretely how the cache works, but just to show that a processor is safe
+/// regardless of the specific cache policy in use.
+///
+/// We do this by defining a type of function, a *cache policy*, that indicates
+/// what a given memory operation does to the cache.
+type cache_policy (n:memory_size) =
+       (cache_state n) -> memory_operation -> (cache_state n)
+
+/// As usual, we define an equivalence relation on memory operations so that
+/// we can determine whether they leak information.  In this case, we say that
+/// two memory operations are equivalent if they load/store the same register
+/// to the same address:
+let equiv_memory_operation (lhs rhs: memory_operation) =
+  match lhs, rhs with
+    | (Load la ld), (Load ra rd) -> (la = ra /\ ld = rd)
+    | (Store la ls), (Store ra rs) -> (la = ra /\ ls = rs)
+    | _, _ -> False
+
+/// We also define equivalence of lists of memory operations, since an
+/// instruction might perform several memory operations.
+let rec equiv_memory_operations (lhs rhs: list memory_operation) =
+  match lhs, rhs with
+    | lh :: lt, rh :: rt -> (equiv_memory_operation lh rh) /\ equiv_memory_operations lt rt
+    | [], [] -> True
+    | _, _ -> False
+
+/// Then we prove various properties of these relations:
+///  - **Equality implies equivalence**:
+let equal_memory_operations_are_equivalent (lhs rhs: memory_operation):
+  Lemma (requires lhs = rhs)
+        (ensures  (equiv_memory_operation lhs rhs)) =
+  ()
+
+let rec equal_memory_operation_lists_are_equivalent (lhs rhs: list memory_operation):
+  Lemma (requires lhs = rhs)
+        (ensures equiv_memory_operations lhs rhs) =
+  match lhs, rhs with
+    | hl :: tl, hr :: tr -> (
+         equal_memory_operations_are_equivalent hl hr;
+         equal_memory_operation_lists_are_equivalent tl tr
+      )
+    | _ -> ()
+
+///  - **Symmetry**
+let memory_operation_equivalence_is_symmetric (lhs rhs: memory_operation):
+  Lemma (requires (equiv_memory_operation lhs rhs))
+        (ensures  (equiv_memory_operation rhs lhs)) =
+  ()
+
+let rec memory_operation_list_equivalence_is_symmetric (lhs rhs: list memory_operation):
+  Lemma (requires (equiv_memory_operations lhs rhs))
+        (ensures  (equiv_memory_operations rhs lhs)) =
+  match lhs, rhs with
+   | hl :: tl, hr :: tr -> (
+        memory_operation_equivalence_is_symmetric hl hr;
+        memory_operation_list_equivalence_is_symmetric tl tr
+     )
+   | _ -> ()
+
+///  - **Transitivity**
+let memory_operation_equivalence_is_transitive (lhs mid rhs: memory_operation):
+  Lemma (requires (equiv_memory_operation lhs mid) /\ (equiv_memory_operation mid rhs))
+        (ensures  (equiv_memory_operation lhs rhs)) =
+  ()
+
+let rec memory_operation_list_equivalence_is_transitive (lhs mid rhs: list memory_operation):
+  Lemma (requires (equiv_memory_operations lhs mid) /\ (equiv_memory_operations mid rhs))
+        (ensures  (equiv_memory_operations lhs rhs)) =
+  match lhs, mid, rhs with
+   | hl :: tl, hm :: tm, hr :: tr -> (
+        memory_operation_equivalence_is_transitive hl hm hr;
+        memory_operation_list_equivalence_is_transitive tl tm tr
+     )
+   | _ -> ()
+
+///  - **Equivalence of lists implies equality of length**
+let rec equivalent_memory_operation_lists_have_equal_length (lhs rhs: list memory_operation):
+  Lemma (requires equiv_memory_operations lhs rhs)
+        (ensures (FStar.List.length lhs) = (FStar.List.length rhs)) =
+  match lhs, rhs with
+    | hl :: tl, hr :: tr -> equivalent_memory_operation_lists_have_equal_length tl tr
+    | _, _ -> ()
+
+
+/// Next, we look at how to actually complete the transactions.  A load
+/// results in the register file being updated with a value from memory.
+/// A store results in memory being updated with a value from the register
+/// file.
+let complete_one_memory_transaction (#n #r: memory_size)
+    (op:memory_operation) (pre:systemState #n #r) (cp:cache_policy n): systemState #n #r =
+  match op with
+      | Load address register ->
+             if register < FStar.List.length pre.registers
+                  && address < FStar.List.length pre.memory then
+                { pre with registers = replace_list_value
+                                         pre.registers
+                                         register
+                                         (FStar.List.Tot.index pre.memory address);
+                           cache_lines = cp pre.cache_lines op }
+             else pre
+      | Store address register ->
+             if register < FStar.List.length pre.registers
+                  && address < FStar.List.length pre.memory then
+                { pre with memory = replace_list_value
+                                      pre.memory
+                                      address
+                                      (FStar.List.Tot.index pre.registers register);
+                           cache_lines = cp pre.cache_lines op }
+             else pre
+
+let rec complete_memory_transactions (#n #r: memory_size)
+    (op:list memory_operation) (pre:systemState #n #r) (cp:cache_policy n) =
   match op with
     | hd :: tl -> (let post = (complete_one_memory_transaction hd pre cp) in
                  complete_memory_transactions tl post cp)
     | [] -> pre
 
+/// Then, we show that our notion of equivalence of memory operations leads
+/// to the conclusion that applying equivalent operations to equivalent systems
+/// yields equivalent systems.
 let completing_single_memory_transactions_on_equivalent_systems_yields_equivalent_systems
     (#m #q #n #r: memory_size)
-    (op1:storage_operation) (op2:storage_operation)
+    (op1:memory_operation) (op2:memory_operation)
     (state1:systemState #m #q) (state2 :systemState #n #r)
     (cp:cache_policy m):
-    Lemma (requires (equiv_system state1 state2) /\ (equiv_storage_operation op1 op2))
-          (ensures  (equiv_system (complete_one_memory_transaction op1 state1 cp) (complete_one_memory_transaction op2 state2 cp))) =
+    Lemma (requires (equiv_system state1 state2) /\ (equiv_memory_operation op1 op2))
+          (ensures  (equiv_system (complete_one_memory_transaction op1 state1 cp)
+                                  (complete_one_memory_transaction op2 state2 cp))) =
                  let post1 = (complete_one_memory_transaction op1 state1 cp) in
                  let post2 = (complete_one_memory_transaction op2 state2 cp) in
 
@@ -449,23 +457,29 @@ let completing_single_memory_transactions_on_equivalent_systems_yields_equivalen
                          assert(equiv_list state1.memory    state2.memory);
 
 
-                         if (a1 < FStar.List.length state1.memory) && (r1 < FStar.List.length state1.registers) then (
+                         if (a1 < FStar.List.length state1.memory)
+                                && (r1 < FStar.List.length state1.registers) then (
 
                            assert(a2 < FStar.List.length state2.memory);
                            assert(r2 < FStar.List.length state2.registers);
 
-                           equivalent_lists_have_equivalent_values word state1.memory state2.memory a1;
+                           equivalent_lists_have_equivalent_values
+                             word state1.memory state2.memory a1;
+
                            let write1 = (FStar.List.Tot.index state1.memory a1) in
                            let write2 = (FStar.List.Tot.index state2.memory a2) in
                            assert(equiv write1 write2);
 
                            assert(post1.registers = (replace_list_value state1.registers r1 write1));
                            assert(post2.registers = (replace_list_value state2.registers r2 write2));
-                           replacing_in_equivalent_lists_with_equivalent_value_yields_equivalent_lists state1.registers state2.registers r1 write1 write2;
+
+                           replacing_in_equivalent_lists_with_equivalent_value_yields_equivalent_lists
+                             state1.registers state2.registers r1 write1 write2;
+
                            assert(equiv_list post1.registers post2.registers);
                            assert(equiv_list state1.memory state2.memory);
                            assert(post1.pc = post2.pc)
-                           )
+                         )
                          else (
                            assert(post1 = state1);
                            assert(post2 = state2)
@@ -479,19 +493,25 @@ let completing_single_memory_transactions_on_equivalent_systems_yields_equivalen
                          assert(equiv_list state1.registers state2.registers);
                          assert(equiv_list state1.memory    state2.memory);
 
-                         if (a1 < FStar.List.length state1.memory) && (r1 < FStar.List.length state1.registers) then (
+                         if (a1 < FStar.List.length state1.memory)
+                                && (r1 < FStar.List.length state1.registers) then (
 
                            assert(a2 < FStar.List.length state2.memory);
                            assert(r2 < FStar.List.length state2.registers);
 
-                           equivalent_lists_have_equivalent_values word state1.registers state2.registers r1;
+                           equivalent_lists_have_equivalent_values
+                             word state1.registers state2.registers r1;
+
                            let write1 = (FStar.List.Tot.index state1.registers r1) in
                            let write2 = (FStar.List.Tot.index state2.registers r2) in
                            assert(equiv write1 write2);
 
                            assert(post1.memory = (replace_list_value state1.memory a1 write1));
                            assert(post2.memory = (replace_list_value state2.memory a2 write2));
-                           replacing_in_equivalent_lists_with_equivalent_value_yields_equivalent_lists state1.memory state2.memory a1 write1 write2;
+
+                           replacing_in_equivalent_lists_with_equivalent_value_yields_equivalent_lists
+                             state1.memory state2.memory a1 write1 write2;
+
                            assert(equiv_list post1.registers post2.registers);
                            assert(equiv_list state1.memory state2.memory);
                            assert(post1.pc = post2.pc)
@@ -506,110 +526,219 @@ let completing_single_memory_transactions_on_equivalent_systems_yields_equivalen
 
 let rec completing_equivalent_memory_transactions_on_equivalent_systems_yields_equivalent_systems
     (#m #q #n #r: memory_size)
-    (ops1:list storage_operation) (ops2:(list storage_operation){FStar.List.length ops1 = FStar.List.length ops2})
+    (ops1:list memory_operation)
+    (ops2:(list memory_operation){FStar.List.length ops1 = FStar.List.length ops2})
     (state1:systemState #m #q) (state2 :systemState #n #r)
     (cp: cache_policy m):
-    Lemma (requires (equiv_system state1 state2) /\ (equiv_storage_operations ops1 ops2))
-          (ensures  (equiv_system (complete_memory_transactions ops1 state1 cp) (complete_memory_transactions ops2 state2 cp))) =
+    Lemma (requires (equiv_system state1 state2) /\ (equiv_memory_operations ops1 ops2))
+          (ensures  (equiv_system (complete_memory_transactions ops1 state1 cp)
+                                  (complete_memory_transactions ops2 state2 cp))) =
     assert(m = n /\ q = r);
     match ops1, ops2 with
      | op1 :: t1, op2 :: t2 -> (
            let post1 = complete_one_memory_transaction op1 state1 cp in
            let post2 = complete_one_memory_transaction op2 state2 cp in
-           completing_single_memory_transactions_on_equivalent_systems_yields_equivalent_systems op1 op2 state1 state2 cp;
-           completing_equivalent_memory_transactions_on_equivalent_systems_yields_equivalent_systems t1 t2 post1 post2 cp
+           completing_single_memory_transactions_on_equivalent_systems_yields_equivalent_systems
+             op1 op2 state1 state2 cp;
+
+           completing_equivalent_memory_transactions_on_equivalent_systems_yields_equivalent_systems
+             t1 t2 post1 post2 cp
        )
      | [], [] -> ()
 
-let rec any_value_is_blinded (values: list (maybeBlinded #word)): bool =
-  match values with
-    | Nil              -> false
-    | Blinded(hd) :: _  -> true
-    | Clear(hd)   :: tl -> any_value_is_blinded tl
+/// ============
+/// Instructions
+/// ============
+///
+/// The next step is to define the concept of an instruction decoding.  We
+/// don't want to analyze a specific ISA here, so instead we suppose that there
+/// is an instruction decoder in the processor that will identify the instruction
+/// operands before execution.
 
-let rec equivalent_memories_have_identical_any_blindedness (a b: list (maybeBlinded #word)):
-  Lemma (requires (equiv_list a b))
-        (ensures (any_value_is_blinded a) = (any_value_is_blinded b))
-  = match a, b with
-      | hl::tl, hr::tr -> equivalent_memories_have_identical_any_blindedness tl tr
-      | _ -> ()
-
-let rec blind_all_values (values: list (maybeBlinded #word)): r:(list (maybeBlinded #word)){FStar.List.length values = FStar.List.length r} =
-    match values with
-      | Nil              -> Nil
-      | Blinded(hd) :: tl -> Blinded(hd) :: blind_all_values tl
-      | Clear(hd)   :: tl -> Blinded(hd) :: blind_all_values tl
-
-let rec blinding_all_values_blinds_each_value (values: list (maybeBlinded #word)) (n:nat{n < FStar.List.length values}):
-  Lemma (ensures Blinded? (FStar.List.Tot.index (blind_all_values values) n))
-        [SMTPat (Blinded? (FStar.List.Tot.index (blind_all_values values) n))] =
-  match n, values with
-    | 0, _   -> ()
-    | _, Nil -> ()
-    | n, hd :: tl -> blinding_all_values_blinds_each_value tl (n-1)
+type decodedInstruction = { opcode: nat; input_operands: list operand; output_operands: list operand }
+type decoder = (inst:word) -> decodedInstruction
+type decoder_output (d:decoder) = (di:decodedInstruction{exists(inst:word). di = d inst})
 
 
-let rec blinding_all_values_is_idempotent (values: list (maybeBlinded #word)):
-  Lemma (ensures (blind_all_values values) = blind_all_values (blind_all_values values)) =
-    match values with
-      | hd :: tl -> blinding_all_values_is_idempotent tl
-      | _ -> ()
+/// -------
+/// Outputs
+/// -------
+///
+/// Once we know what the instruction operands are, we can define a
+/// representation of the results of the instruction.  This contains a value
+/// corresponding to each output operand (as identified by the instruction
+/// decoder), as well as a list of memory operations.
+type instruction_result (di:decodedInstruction) = {
+  register_writes: (vals:(list (maybeBlinded #word)){
+                     FStar.List.length vals = FStar.List.length di.output_operands});
+  memory_ops: (list memory_operation)
+}
 
-let rec blinding_all_values_blinds_all_values (values: list (maybeBlinded #word)):
-  Lemma (ensures all_values_are_blinded _ (blind_all_values values))
-        [SMTPat (blind_all_values values)] =
-  match values with
-    | hd :: tl -> blinding_all_values_blinds_all_values tl
-    | _ -> ()
+/// We can then define an equivalence relation on instruction results to see
+/// whether they leak information:
+let equiv_result (#di:decodedInstruction) (lhs rhs:(instruction_result di)) =
+    (equiv_list lhs.register_writes rhs.register_writes)
+  /\ (equiv_memory_operations lhs.memory_ops rhs.memory_ops)
 
-let rec equivalent_unblinded_lists_are_equal (a b: list (maybeBlinded #word)):
-  Lemma (requires (equiv_list a b) /\ (~(any_value_is_blinded a) \/ ~(any_value_is_blinded b)))
-        (ensures a = b) =
-  match a, b with
-    | h1 :: t1, h2 :: t2 -> equivalent_unblinded_lists_are_equal t1 t2
-    | _ -> ()
+/// Then we define the usual bevy of properties:
+///  - **Equality implies equivalence**:
+let equal_results_are_equivalent (#di:decodedInstruction) (lhs rhs:(instruction_result di)):
+  Lemma (requires lhs = rhs)
+        (ensures  equiv_result lhs rhs)
+  = equal_lists_are_equivalent word lhs.register_writes rhs.register_writes;
+    equal_memory_operation_lists_are_equivalent lhs.memory_ops rhs.memory_ops
 
-let rec mux_list (a:list (maybeBlinded #word)) (b:(list (maybeBlinded #word))) (which_b:list nat): Tot (list (maybeBlinded #word)) (decreases which_b) =
-  match which_b with
-    | Nil -> a
-    | index_to_change :: tl -> mux_list (mux_list_single a b index_to_change) b tl
+///  - **Symmetry**
+let result_equivalence_is_symmetric (#di:decodedInstruction) (lhs rhs:(instruction_result di)):
+  Lemma (requires equiv_result lhs rhs)
+        (ensures equiv_result rhs lhs) =
+  list_equivalence_is_symmetric word lhs.register_writes rhs.register_writes;
+  memory_operation_list_equivalence_is_symmetric lhs.memory_ops rhs.memory_ops
+
+///  - **Transitivity**
+let result_equivalence_is_transitive (#di:decodedInstruction) (lhs mid rhs:(instruction_result di)):
+  Lemma (requires (equiv_result lhs mid) /\ (equiv_result mid rhs))
+        (ensures  (equiv_result lhs rhs)) =
+  list_equivalence_is_transitive word lhs.register_writes mid.register_writes rhs.register_writes;
+  memory_operation_list_equivalence_is_transitive lhs.memory_ops mid.memory_ops rhs.memory_ops
+
+/// ------
+/// Inputs
+/// ------
+///
+/// We also define a type that indicates which lists of input operands are
+/// compatible with a decoded instruction: some lists are just not possible,
+/// either because they have the wrong number of operands for that instruction,
+/// or because they conflict with each other (e.g. r1, r2, r1 → 1, 2, 3).
+type instruction_input (#n #r: memory_size) (di:decodedInstruction) =
+     pre:(list (maybeBlinded #word)){
+           (exists(s: systemState #n #r). pre = get_operands di.input_operands s)
+                 /\ FStar.List.length pre = FStar.List.length di.input_operands}
+
+/// We then show that this property is preserved by redaction.
+let redacted_instruction_inputs_are_instruction_inputs  (#n #r: memory_size)
+    (di:decodedInstruction) (pre:instruction_input #n #r di): instruction_input #n #r di
+  = assert(exists (s:systemState). (pre = get_operands #n #r di.input_operands s /\
+                                 (get_operands #n #r di.input_operands (redact_system s)
+                   = redact_list (get_operands di.input_operands s) 0uL  )  ) );
+    redact_list pre 0uL
+
+/// ---------
+/// Semantics
+/// ---------
+///
+/// Next we start looking at what the instructions actually do.  Earlier we
+/// defined the idea of an :ref:`execution unit <execution_unit>` that maps
+/// an old state to a new state according to an instruction.  Now we want do
+/// define an equivalent mapping, but in terms of instruction inputs and
+/// outputs:
+type instruction_semantics (#n #r: memory_size) (d:decoder) =
+  (di: decoder_output d) -> (pre:instruction_input #n #r di) -> instruction_result di
+
+/// We can define a notion of redacting-equivalence for the instruction semantics too.
+let is_redacting_equivalent_instruction_semantics_somewhere
+      (#n #r: memory_size)
+      (d:decoder)
+      (s:instruction_semantics #n #r d)
+      (inst:word)
+      (input:instruction_input #n #r (d inst)) =
+    redaction_preserves_length word input 0uL;
+    let redacted_input = redacted_instruction_inputs_are_instruction_inputs (d inst) input in
+    (equiv_result (s (d inst) input) (s (d inst) redacted_input))
+
+let is_redacting_equivalent_instruction_semantics_everywhere (#n #r: memory_size)
+    (d:decoder) (s:instruction_semantics #n #r d)
+    = forall (inst:word) (pre:instruction_input #n #r (d inst)).
+                is_redacting_equivalent_instruction_semantics_somewhere d s inst pre
+
+/// Then as before, we show that redacting-equivalent instruction semantics
+/// lead to equivalent results when applied to a redacted input.
+let redacting_equivalent_instruction_semantics_on_equivalent_inputs_yields_equivalent_results_somewhere
+      (#n #r: memory_size)
+      (d:decoder)
+      (s:instruction_semantics #n #r d)
+      (inst:word)
+      (input1 input2:instruction_input #n #r (d inst)):
+  Lemma (requires (is_redacting_equivalent_instruction_semantics_everywhere d s)
+                  /\ (equiv_list input1 input2))
+        (ensures  equiv_result (s (d inst) input1) (s (d inst) input2)) =
+  let result1 = (s (d inst) input1) in
+  let result2 = (s (d inst) input2) in
+  let redacted_result1 = (s (d inst) (redact_list input1 0uL)) in
+  let redacted_result2 = (s (d inst) (redact_list input2 0uL)) in
+
+  equivalent_lists_have_equal_redactions word input1 input2 0uL;
+  assert(redacted_result1 = redacted_result2);
+  equal_results_are_equivalent redacted_result1 redacted_result2;
+
+  result_equivalence_is_symmetric result2 redacted_result1;
+
+  assert(equiv_result result1 redacted_result1);
+  assert(equiv_result redacted_result1 result2);
+
+  result_equivalence_is_transitive result1 redacted_result1 result2;
+  assert(equiv_result result1 result2)
+
 
 /// ===============
 /// Execution model
 /// ===============
-
-let decoding_execution_unit (#n #r: memory_size) (d:decoder) (s:instruction_semantics #n #r d)  (cp: cache_policy n) (inst:word) (pre:systemState #n #r): systemState #n #r =
+///
+/// We now define the :ref:`execution unit <execution_unit>` in terms of an instruction
+/// semantics function.  This execution unit
+///
+/// #. decodes the instruction,
+/// #. reads the input operands from the register file,
+/// #. performs the computation,
+/// #. increments the program counter, and
+/// #. writes the result to the system's register file.
+///
+let decoding_execution_unit (#n #r: memory_size)
+    (d:decoder) (s:instruction_semantics #n #r d) (cp: cache_policy n)
+    (inst:word) (pre:systemState #n #r): systemState #n #r =
     let decoded = d inst in
     let input_operand_values = (get_operands decoded.input_operands pre) in
     let instruction_output = (s decoded input_operand_values) in
     let output_operand_values = instruction_output.register_writes in
-    let pre_with_incremented_pc = { pre with pc = (
-                                        if FStar.UInt64.v pre.pc < FStar.List.length pre.memory - 1 then
-                                          FStar.UInt64.add pre.pc 1uL
-                                        else
-                                          0uL
-                                        ) } in
-    let intermediate_with_updated_registers = set_operands decoded.output_operands output_operand_values pre_with_incremented_pc in
+    let pre_with_incremented_pc =
+          { pre with pc = (
+                if FStar.UInt64.v pre.pc < FStar.List.length pre.memory - 1
+                then
+                  FStar.UInt64.add pre.pc 1uL
+                else
+                  0uL
+            ) } in
+    let intermediate_with_updated_registers =
+      set_operands decoded.output_operands output_operand_values pre_with_incremented_pc in
     complete_memory_transactions instruction_output.memory_ops intermediate_with_updated_registers cp
 
-/// ==================
-/// Safety definitions
-/// ==================
-
-irreducible let trigger (#n #r: memory_size) (d:decoder) (s:instruction_semantics #n #r d) (cp:cache_policy n) (inst:word) (pre:systemState #n #r) = False
+/// We need this for technical reasons, to trigger the inclusion of some lemmas
+/// into the proof state.
+irreducible let trigger (#n #r: memory_size)
+  (d:decoder) (s:instruction_semantics #n #r d) (cp:cache_policy n)
+  (inst:word) (pre:systemState #n #r) = False
 
 
 /// ---------------------------
 /// Redacting-equivalent safety
 /// ---------------------------
-let decoding_execution_unit_with_redacting_equivalent_instruction_semantics_is_redacting_equivalent_somewhere (#n #r: memory_size) (d:decoder) (s:(instruction_semantics #n #r d){is_redacting_equivalent_instruction_semantics_everywhere d s}) (cp:cache_policy n) (inst:word) (pre:systemState #n #r):
+///
+/// Now we are at the point that we can start to prove security properties of this execution unit, when applied to instruction semantics that are also redacting-equivalent.
+///
+/// First, that it is redacting equivalent for specific instructions and system states.
+let decoding_execution_unit_with_re_instruction_semantics_is_redacting_equivalent_somewhere
+      (#n #r: memory_size)
+      (d:decoder)
+      (s:(instruction_semantics #n #r d){is_redacting_equivalent_instruction_semantics_everywhere d s})
+      (cp:cache_policy n)
+      (inst:word)
+      (pre:systemState #n #r):
     Lemma (ensures (equiv_system (decoding_execution_unit d s cp inst pre)
                                  (decoding_execution_unit d s cp inst (redact_system pre))))
     [SMTPat (trigger d s cp inst pre)] =
       let decoded = d inst in
       let input_operand_values = (get_operands decoded.input_operands pre) in
       let redacted_input_operand_values = (get_operands decoded.input_operands (redact_system pre)) in
-      (* let redacted_input_operand_values = (redact_list (get_operands decoded.input_operands pre) 0) in *)
       let instruction_output = (s decoded input_operand_values) in
       let redacted_instruction_output = (s decoded redacted_input_operand_values) in
       let pre_with_incremented_pc = { pre with pc = (
@@ -620,23 +749,38 @@ let decoding_execution_unit_with_redacting_equivalent_instruction_semantics_is_r
                                       ) } in
 
       systems_are_equivalent_to_their_redaction pre;
-      get_operands_on_equivalent_inputs_has_equivalent_output decoded.input_operands pre (redact_system pre);
+
+      get_operands_on_equivalent_inputs_has_equivalent_output
+        decoded.input_operands
+        pre
+        (redact_system pre);
+
       assert(equiv_list input_operand_values redacted_input_operand_values);
 
-      redacting_equivalent_instruction_semantics_on_equivalent_inputs_yields_equivalent_results_somewhere d s inst input_operand_values redacted_input_operand_values;
+      redacting_equivalent_instruction_semantics_on_equivalent_inputs_yields_equivalent_results_somewhere
+        d s inst input_operand_values redacted_input_operand_values;
+
       assert(equiv_result instruction_output redacted_instruction_output);
 
       lists_are_equivalent_to_their_redaction word input_operand_values 0uL;
 
       assert(equiv_list input_operand_values (get_operands decoded.input_operands (redact_system pre)));
 
-      list_equivalence_is_transitive word redacted_input_operand_values input_operand_values (get_operands decoded.input_operands (redact_system pre));
-      assert(equiv_list redacted_input_operand_values (get_operands decoded.input_operands (redact_system pre)));
+      list_equivalence_is_transitive word redacted_input_operand_values
+        input_operand_values
+        (get_operands decoded.input_operands (redact_system pre));
+
+      assert(equiv_list redacted_input_operand_values
+                        (get_operands decoded.input_operands (redact_system pre)));
 
       assert(equiv_list instruction_output.register_writes redacted_instruction_output.register_writes);
 
-      let post1 = set_operands decoded.output_operands instruction_output.register_writes pre_with_incremented_pc in
-      let post_redacted1 = set_operands decoded.output_operands redacted_instruction_output.register_writes (redact_system pre_with_incremented_pc) in
+      let post1 = set_operands decoded.output_operands
+                               instruction_output.register_writes
+                               pre_with_incremented_pc in
+      let post_redacted1 = set_operands decoded.output_operands
+                                        redacted_instruction_output.register_writes
+                                        (redact_system pre_with_incremented_pc) in
 
       systems_are_equivalent_to_their_redaction pre_with_incremented_pc;
       assert(equiv_system pre_with_incremented_pc (redact_system pre_with_incremented_pc));
@@ -649,11 +793,16 @@ let decoding_execution_unit_with_redacting_equivalent_instruction_semantics_is_r
 
       assert(equiv_system post1 post_redacted1);
 
-      let post2: systemState #n #r = complete_memory_transactions instruction_output.memory_ops post1 cp in
-      let post_redacted2: systemState #n #r = complete_memory_transactions redacted_instruction_output.memory_ops post_redacted1 cp in
+      let post2: systemState #n #r = complete_memory_transactions instruction_output.memory_ops
+                                                                  post1
+                                                                  cp in
+      let post_redacted2: systemState #n #r =
+        complete_memory_transactions redacted_instruction_output.memory_ops post_redacted1 cp in
 
-      assert(equiv_storage_operations instruction_output.memory_ops redacted_instruction_output.memory_ops);
-      equivalent_storage_operation_lists_have_equal_length instruction_output.memory_ops redacted_instruction_output.memory_ops;
+      assert(equiv_memory_operations instruction_output.memory_ops
+                                     redacted_instruction_output.memory_ops);
+      equivalent_memory_operation_lists_have_equal_length
+        instruction_output.memory_ops redacted_instruction_output.memory_ops;
 
       completing_equivalent_memory_transactions_on_equivalent_systems_yields_equivalent_systems
         instruction_output.memory_ops
@@ -664,18 +813,28 @@ let decoding_execution_unit_with_redacting_equivalent_instruction_semantics_is_r
 
       assert(equiv_system post2 post_redacted2)
 
-let decoding_execution_unit_with_redacting_equivalent_instruction_semantics_is_redacting_equivalent (#n #r: memory_size) (d:decoder) (s:(instruction_semantics #n #r d){is_redacting_equivalent_instruction_semantics_everywhere d s}) (cp:cache_policy n):
+/// Next, that it is redacting equivalent for all instructions and system states.
+let decoding_execution_unit_with_re_instruction_semantics_is_redacting_equivalent
+    (#n #r: memory_size)
+    (d:decoder)
+    (s:(instruction_semantics #n #r d){is_redacting_equivalent_instruction_semantics_everywhere d s})
+    (cp:cache_policy n):
   Lemma (ensures forall(pre:systemState #n #r) (inst:word).
                  (equiv_system (decoding_execution_unit d s cp inst pre)
                                (decoding_execution_unit d s cp inst (redact_system pre)))
                  \/ (trigger d s cp inst pre) )
     = ()
 
+/// -------------------
+/// Main safety theorem
+/// -------------------
 
-/// ------------
-/// Main theorem
-/// ------------
-let each_decoding_execution_unit_with_redacting_equivalent_instruction_semantics_is_safe (#n #r: memory_size) (d:decoder) (s:(instruction_semantics #n #r d){is_redacting_equivalent_instruction_semantics_everywhere d s}) (cp:cache_policy n):
+/// Finally, we show that the decoding execution unit is safe.
+let each_decoding_execution_unit_with_redacting_equivalent_instruction_semantics_is_safe
+      (#n #r: memory_size)
+      (d:decoder)
+      (s:(instruction_semantics #n #r d){is_redacting_equivalent_instruction_semantics_everywhere d s})
+      (cp:cache_policy n):
   Lemma (ensures is_safe (decoding_execution_unit d s cp))
-  = decoding_execution_unit_with_redacting_equivalent_instruction_semantics_is_redacting_equivalent d s cp;
+  = decoding_execution_unit_with_re_instruction_semantics_is_redacting_equivalent d s cp;
     redacting_equivalent_execution_units_are_safe (decoding_execution_unit d s cp)
